
\documentclass{article}
%%%%%%%%%%%%%%%%%%%%%%%%%%%%%%%%%%%%%%%%%%%%%%%%%%%%%%%%%%%%%%%%%%%%%%%%%%%%%%%%%%%%%%%%%%%%%%%%%%%%%%%%%%%%%%%%%%%%%%%%%%%%%%%%%%%%%%%%%%%%%%%%%%%%%%%%%%%%%%%%%%%%%%%%%%%%%%%%%%%%%%%%%%%%%%%%%%%%%%%%%%%%%%%%%%%%%%%%%%%%%%%%%%%%%%%%%%%%%%%%%%%%%%%%%%%%
%TCIDATA{OutputFilter=LATEX.DLL}
%TCIDATA{Version=5.50.0.2953}
%TCIDATA{<META NAME="SaveForMode" CONTENT="1">}
%TCIDATA{BibliographyScheme=Manual}
%TCIDATA{Created=Tuesday, January 25, 2022 15:01:52}
%TCIDATA{LastRevised=Tuesday, January 25, 2022 21:15:49}
%TCIDATA{<META NAME="GraphicsSave" CONTENT="32">}
%TCIDATA{<META NAME="DocumentShell" CONTENT="Standard LaTeX\Blank - Standard LaTeX Article">}
%TCIDATA{CSTFile=40 LaTeX article.cst}
%TCIDATA{ComputeDefs=
%$f(x)=e^{x^{2}}$
%$g(x)=e^{-x}$
%}


\newtheorem{theorem}{Theorem}
\newtheorem{acknowledgement}[theorem]{Acknowledgement}
\newtheorem{algorithm}[theorem]{Algorithm}
\newtheorem{axiom}[theorem]{Axiom}
\newtheorem{case}[theorem]{Case}
\newtheorem{claim}[theorem]{Claim}
\newtheorem{conclusion}[theorem]{Conclusion}
\newtheorem{condition}[theorem]{Condition}
\newtheorem{conjecture}[theorem]{Conjecture}
\newtheorem{corollary}[theorem]{Corollary}
\newtheorem{criterion}[theorem]{Criterion}
\newtheorem{definition}[theorem]{Definition}
\newtheorem{example}[theorem]{Example}
\newtheorem{exercise}[theorem]{Exercise}
\newtheorem{lemma}[theorem]{Lemma}
\newtheorem{notation}[theorem]{Notation}
\newtheorem{problem}[theorem]{Problem}
\newtheorem{proposition}[theorem]{Proposition}
\newtheorem{remark}[theorem]{Remark}
\newtheorem{solution}[theorem]{Solution}
\newtheorem{summary}[theorem]{Summary}
\newenvironment{proof}[1][Proof]{\noindent\textbf{#1.} }{\ \rule{0.5em}{0.5em}}
\input{tcilatex}

\begin{document}


\section{1}

1.

$g(x)=e^{-x}$

\begin{tabular}{lll}
$g(x)=\allowbreak e^{-x}$ & $\rightarrow $ & $g(0)=\allowbreak \allowbreak 1$
\\ 
$g^{\prime }(x)=-e^{-x}$ & $\rightarrow $ & $g^{\prime }(0)=\allowbreak -1$
\\ 
$g^{\prime \prime }(x)=\allowbreak e^{-x}$ & $\rightarrow $ & $g^{\prime
\prime }(0)=\allowbreak \allowbreak 1$ \\ 
$g^{\prime \prime \prime }(x)=\allowbreak \allowbreak -e^{-x}$ & $%
\rightarrow $ & $g^{\prime \prime \prime }(0)=\allowbreak \allowbreak -1$ \\ 
$g^{(4)}(x)=\allowbreak e^{-x}$ & $\rightarrow $ & $g^{(4)}(0)=\allowbreak 1$
\\ 
$g^{(5)}(x)=\allowbreak -e^{-x}$ & $\rightarrow $ & $g^{(5)}(0)=\allowbreak
-1$ \\ 
$g^{(6)}(x)=\allowbreak e^{-x}$ & $\rightarrow $ & $g^{(6)}(0)=\allowbreak
\allowbreak 1$ \\ 
$g^{(7)}(x)=\allowbreak \allowbreak -e^{-x}$ & $\rightarrow $ & $%
g^{(7)}(0)=\allowbreak -1$ \\ 
$g^{(8)}(x)=\allowbreak \allowbreak e^{-x}$ & $\rightarrow $ & $%
g^{(8)}(0)=\allowbreak 1$%
\end{tabular}

$e^{-x}=1-\frac{1}{1!}x+\frac{1}{2!}x^{2}-\frac{1}{3!}x^{3}+\frac{1}{4!}%
x^{4}-...$

$e^{-x}=\sum_{n=0}^{\infty }\frac{(-1)^{n}}{n!}x^{n}$\newline

metodo 1:

$1-x+\frac{x^{2}}{2}-\frac{x^{3}}{3!}+\frac{x^{4}}{4!}-\frac{x^{5}}{5!}+%
\frac{x^{6}}{6!}-\frac{x^{7}}{7!}+\frac{x^{8}}{8!}-\frac{x^{9}}{9!}+\frac{%
x^{10}}{10!}-\frac{x^{11}}{11!}+\frac{x^{12}}{12!}-\frac{x^{13}}{13!}+\frac{%
x^{14}}{14!}-\frac{x^{15}}{15!}+\frac{x^{16}}{16!}-\frac{x^{17}}{17!}+\frac{%
x^{18}}{18!}-\frac{x^{19}}{19!}+\frac{x^{20}}{20!}$

sustiticion

$1-5+\frac{5^{2}}{2}-\frac{5^{3}}{3!}+\frac{5^{4}}{4!}-\frac{5^{5}}{5!}+%
\frac{5^{6}}{6!}-\frac{5^{7}}{7!}+\frac{5^{8}}{8!}-\frac{5^{9}}{9!}+\frac{%
5^{10}}{10!}-\frac{5^{11}}{11!}+\frac{5^{12}}{12!}-\frac{5^{13}}{13!}+\frac{%
5^{14}}{14!}-\frac{5^{15}}{15!}+\frac{5^{16}}{16!}-\frac{5^{17}}{17!}+\frac{%
5^{18}}{18!}-\frac{5^{19}}{19!}+\frac{5^{20}}{20!}=\allowbreak \frac{%
26\,257\,\allowbreak 980\,879\,929}{3892\,643\,\allowbreak 213\,082\,624}%
=\allowbreak 6.\,\allowbreak 745\,540\,10\times 10^{-3}$

metodo 2:

$\frac{1}{1-x+\frac{x^{2}}{2}-\frac{x^{3}}{3!}+\frac{x^{4}}{4!}-\frac{x^{5}}{%
5!}+\frac{x^{6}}{6!}-\frac{x^{7}}{7!}+\frac{x^{8}}{8!}-\frac{x^{9}}{9!}+%
\frac{x^{10}}{10!}-\frac{x^{11}}{11!}+\frac{x^{12}}{12!}-\frac{x^{13}}{13!}+%
\frac{x^{14}}{14!}-\frac{x^{15}}{15!}+\frac{x^{16}}{16!}-\frac{x^{17}}{17!}+%
\frac{x^{18}}{18!}-\frac{x^{19}}{19!}+\frac{x^{20}}{20!}}$

sustiticion

$\frac{1}{1-5+\frac{5^{2}}{2}-\frac{5^{3}}{3!}+\frac{5^{4}}{4!}-\frac{5^{5}}{%
5!}+\frac{5^{6}}{6!}-\frac{5^{7}}{7!}+\frac{5^{8}}{8!}-\frac{5^{9}}{9!}+%
\frac{5^{10}}{10!}-\frac{5^{11}}{11!}+\frac{5^{12}}{12!}-\frac{5^{13}}{13!}+%
\frac{5^{14}}{14!}-\frac{5^{15}}{15!}+\frac{5^{16}}{16!}-\frac{5^{17}}{17!}+%
\frac{5^{18}}{18!}-\frac{5^{19}}{19!}+\frac{5^{20}}{20!}}=\allowbreak \frac{%
3892\,643\,\allowbreak 213\,082\,624}{26\,257\,\allowbreak 980\,879\,929}%
=\allowbreak 148.\,\allowbreak 246\,098$

Error relativo 1:

$E_{r}=\left\Vert \frac{6.737947\times 10^{-3}-6.\,\allowbreak
745\,540\,10\times 10^{-3}}{6.737947\times 10^{-3}}\right\Vert =\allowbreak
1.\,\allowbreak 126\,915\,96\times 10^{-3}$

Error relativo 2:

$E_{r}=\left\Vert \frac{6.737947\times 10^{-3}-148.\,\allowbreak 246\,098}{%
6.737947\times 10^{-3}}\right\Vert =22000.\,\allowbreak 671\,7$

2.

$%
\begin{tabular}{lll}
$f(x)=e^{x^{2}}$ & $\rightarrow $ & $f(0)=\allowbreak 1$ \\ 
$f^{\prime }(x)=\allowbreak 2xe^{x^{2}}$ & $\rightarrow $ & $f^{\prime
}(0)=\allowbreak 0$ \\ 
$f^{\prime \prime }(x)=\allowbreak 2e^{x^{2}}+4x^{2}e^{x^{2}}$ & $%
\rightarrow $ & $f^{\prime \prime }(0)=\allowbreak 2$ \\ 
$f^{\prime \prime \prime }(x)=\allowbreak 12xe^{x^{2}}+8x^{3}e^{x^{2}}$ & $%
\rightarrow $ & $f^{\prime \prime \prime }(0)=\allowbreak 0$ \\ 
$f^{(4)}(x)=\allowbreak 12e^{x^{2}}+48x^{2}e^{x^{2}}+16x^{4}e^{x^{2}}$ & $%
\rightarrow $ & $f^{(4)}(0)=\allowbreak 12$ \\ 
$f^{(5)}(x)=\allowbreak
120xe^{x^{2}}+160x^{3}e^{x^{2}}+32x^{5}e^{x^{2}}\allowbreak $ & $\rightarrow 
$ & $f^{(5)}(0)=\allowbreak 0$ \\ 
$f^{(6)}(x)=\allowbreak
120e^{x^{2}}+720x^{2}e^{x^{2}}+480x^{4}e^{x^{2}}+\allowbreak 64x^{6}e^{x^{2}}
$ & $\rightarrow $ & $f^{(6)}(0)=\allowbreak 120$ \\ 
$f^{(7)}(x)=\allowbreak
1680xe^{x^{2}}+3360x^{3}e^{x^{2}}+1344x^{5}e^{x^{2}}+\allowbreak
128x^{7}e^{x^{2}}$ & $\rightarrow $ & $f^{(7)}(0)=\allowbreak 0$ \\ 
$f^{(8)}(x)=\allowbreak ...$ & $\rightarrow $ & $f^{(8)}(0)=\allowbreak 1680$%
\end{tabular}%
$

$e^{x^{2}}=1+\frac{0}{1!}x+\frac{2}{2!}x^{2}+\frac{0}{3!}x^{3}+\frac{12}{4!}%
x^{4}+...$

\qquad $=1+\frac{2}{2!}x^{2}+\frac{12}{4!}x^{4}+\frac{120}{6!}x^{6}+\frac{%
1680}{8!}x^{8}+...$

integral no pude completarla :( 

$e^{x^{2}}=\sum_{n=0}^{\infty }\frac{{}}{(2n)!}x^{2n}$\newline

Analisis a 10 terminos

$\int_{1}^{3}\frac{e^{x^{2}}}{x^{2}}dx=\int_{1}^{3}\frac{\sum_{n=0}^{\infty }%
\frac{{}}{(2n)!}x^{2n}}{x^{2}}$

\bigskip $f^{(18)}(0)=\allowbreak 17\,\allowbreak 643\,225\,600$

$=\int_{1}^{3}(\frac{1+\frac{2}{2!}x^{2}+\frac{12}{4!}x^{4}+\frac{120}{6!}%
x^{6}+\frac{1680}{8!}x^{8}+\frac{30240}{10!}x^{10}+\frac{665280}{12!}x^{12}+%
\frac{17297280}{14!}x^{14}+\frac{518918400}{16!}x^{16}+\frac{17643225600}{18!%
}x^{18}}{x^{2}})$

$=\int_{1}^{3}(\frac{1}{x^{2}}+1+\frac{12}{4!}x^{2}+\frac{120}{6!}x^{4}+%
\frac{1680}{8!}x^{6}+\frac{30240}{10!}x^{8}+\frac{665280}{12!}x^{10}+\frac{%
17297280}{14!}x^{12}+\frac{518918400}{16!}x^{14}+\frac{17643225600}{18!}%
x^{16})$

$=\frac{-1}{x}+x+\frac{12}{4!}(\frac{x^{3}}{3})+\frac{120}{6!}(\frac{x^{5}}{5%
})+\frac{1680}{8!}(\frac{x^{7}}{7})+\frac{30240}{10!}(\frac{x^{9}}{9})+\frac{%
665280}{12!}(\frac{x^{11}}{11})+\frac{17297280}{14!}(\frac{x^{13}}{13})+%
\frac{518918400}{16!}(\frac{x^{15}}{15})+\frac{17643225600}{18!}(\frac{x^{17}%
}{17})|_{1}^{3}$

sustituir

$=\frac{-1}{(3)}+(3)+\frac{12}{4!}(\frac{(3)^{3}}{3})+\frac{120}{6!}(\frac{%
(3)^{5}}{5})+\frac{1680}{8!}(\frac{(3)^{7}}{7})+\frac{30240}{10!}(\frac{%
(3)^{9}}{9})+\frac{665280}{12!}(\frac{(3)^{11}}{11})+\frac{17297280}{14!}(%
\frac{(3)^{13}}{13})+\frac{518918400}{16!}(\frac{(3)^{15}}{15})+\frac{%
17643225600}{18!}(\frac{(3)^{17}}{17})=\allowbreak \frac{1407\,668\,593}{%
10\,210\,200}=\allowbreak 137.\,\allowbreak 868\,856$

$=\frac{-1}{(1)}+(1)+\frac{12}{4!}(\frac{(1)^{3}}{3})+\frac{120}{6!}(\frac{%
(1)^{5}}{5})+\frac{1680}{8!}(\frac{(1)^{7}}{7})+\frac{30240}{10!}(\frac{%
(1)^{9}}{9})+\frac{665280}{12!}(\frac{(1)^{11}}{11})+\frac{17297280}{14!}(%
\frac{(1)^{13}}{13})+\frac{518918400}{16!}(\frac{(1)^{15}}{15})+\frac{%
17643225600}{18!}(\frac{(1)^{17}}{17})=\allowbreak \frac{114\,141\,551}{%
551\,350\,800}=\allowbreak 0.207\,021\,648\,\allowbreak $

resultado

$\allowbreak 137.\,\allowbreak 868\,856-0.207\,021\,648\,=\allowbreak
137.\,\allowbreak 661\,834$

Error Porcentual

$E_{\%}=\left\Vert \frac{1.87855248264\times 10^{2}-137.\,\allowbreak
661\,834}{1.87855248264\times 10^{2}}\times 100\right\Vert =\allowbreak
26.\,\allowbreak 719\,197\,2\%$

$1.87855248264\times 10^{2}=\allowbreak 187.\,\allowbreak 855\,248$

3.

promedio

\bigskip $\frac{100.0+98.0+101.0+97.0}{4}=\allowbreak 99.0$

Errores:

\bigskip $E_{a}=\left\Vert 99.0-101.0\right\Vert =\allowbreak 2.0$

$E_{p}=\left\Vert \frac{99.0-101.0}{99.0}\right\Vert \times 100=\allowbreak
2.\,\allowbreak 020\,202\,02\%$

4.

\begin{tabular}{cc}
$f(x)=\frac{e^{x}-1-x}{x^{2}}$ & $P(x)=\frac{1}{2}+\frac{x}{6}+\frac{x^{2}}{%
24}$ \\ 
$f(0.01)=\frac{e^{(0.01)}-1-(0.01)}{(0.01)^{2}}=\allowbreak
0.501\,670\,842\,\allowbreak $ & $P(x)=\frac{1}{2}+\frac{(0.01)}{6}+\frac{%
(0.01)^{2}}{24}=\allowbreak 0.501\,670\,833\,\allowbreak $%
\end{tabular}%
\newline

\end{document}
